Updates Theo's approach. Assumes in bind and lift

newio/DM7.fst
@@ -12,25 +12,39 @@ open DM
 let pdm (a:Type) (wp:hist a) = 
   pre : pure_pre { forall p h. wp p h ==> pre } & (squash pre -> dm a wp)
 
+let get_pre #a #w (t : pdm a w) : Pure pure_pre (requires True) (ensures fun r -> forall post hist. w post hist ==> r) =
+  let (| pre , f |) = t in pre
+
+let get_fun #a #w (t : pdm a w) : Pure (dm a w) (requires get_pre t) (ensures fun _ -> True) =
+  let (| pre, f |) = t in f ()
+
 let pdm_return (a:Type) (x:a) : pdm a (hist_return x) =
  (| True, (fun _ -> dm_return _ x) |)
+
+let rec return_of (x:'a) (f:io 'a) =
+  match f with
+  | Return x' -> x == x'
+  | Call cmd arg k ->
+     exists r'. return_of #'a x (k r')
 
 let pdm_bind (a b:Type)
   (wp1:hist a) (wp2:a -> hist b)
   (f:pdm a wp1) 
   (g:(x:a) -> pdm b (wp2 x)) :
   pdm b (hist_bind wp1 wp2) =
-  let (| fpre, f |) = f in
-  (| fpre, (fun _ -> dm_bind a b wp1 wp2 (f _) (fun x -> 
-    let (| gpre, g |) = g x in 
-    g _)) |)
+  let new_pre = get_pre f /\ (forall x. x `return_of` (get_fun f) ==> get_pre (g x)) in
+  assume (forall p h. hist_bind wp1 wp2 p h ==> new_pre);
+  (| new_pre, 
+     (fun _ -> dm_bind a b wp1 wp2 (get_fun f) (fun x -> 
+       assume (x `return_of` (get_fun f));
+       get_fun (g x))) |)
 
 let pdm_subcomp (a:Type) (wp1:hist a) (wp2:hist a) (f:pdm a wp1) :
   Pure (pdm a wp2)
     (requires (
       (wp2 `hist_ord` wp1)))
     (ensures fun _ -> True) =
-  fun ((| pre, pres |)) -> dm_subcomp a wp1 wp2 (f (| pre, pres |))
+  (| get_pre f, (fun _ -> dm_subcomp a wp1 wp2 (get_fun f)) |)
 
   
 unfold
@@ -67,15 +81,15 @@ effect IO
 
 let lift_pure_pdm (a : Type) 
   (w : pure_wp a)
-  (f:(eqtype_as_type unit -> PURE a w))
-  (pre : pure_pre { forall p h. (wp_lift_pure_hist w) p h ==> pre })
-  (spre:squash pre) : 
-  dm a (wp_lift_pure_hist w) =
+  (f:(eqtype_as_type unit -> PURE a w)) : 
+  pdm a (wp_lift_pure_hist w) =
+  assume (forall (p:hist_post a) h. wp_lift_pure_hist #a w p h ==> as_requires w);
+  admit ();
+  (| as_requires w, (fun _ -> 
     FStar.Monotonic.Pure.elim_pure_wp_monotonicity_forall ();
-    assume (pre == as_requires w);
     let r = f () in
     let r' = dm_return _ r in
-    dm_subcomp _ _ _ r'
+    dm_subcomp _ _ _ r' ) |)
 
 sub_effect PURE ~> IOwp = lift_pure_pdm
   
@@ -102,7 +116,7 @@ let static_cmd
     (requires (fun h -> io_pre cmd argz h))
     (ensures (fun h lt r ->
         lt == [convert_call_to_event cmd argz r])) =
-  IOwp?.reflect (fun _ -> io_call cmd argz)
+  IOwp?.reflect (| True,  (fun _ -> io_call cmd argz) |)
 
 let testStatic3 (fd:file_descr) : IO unit (fun h -> is_open fd h) (fun h lt r -> ~(is_open fd (List.rev lt @ h))) =
   let _ = static_cmd Close fd in
